EthCryptographySpecs/Proofs/Xmss.lean
@@ -1,5 +1,5 @@
 import EthCryptographySpecs.Proofs.Xmss.Types
-import EthCryptographySpecs.Proofs.Xmss.Tweak
+import EthCryptographySpecs.Proofs.Xmss.TweakHash
 import EthCryptographySpecs.Proofs.Xmss.Blake2s
 
 /-!
